stuck

theories/StackMachines/BSM/TM_computable_to_BSM_computable.v
@@ -5,6 +5,7 @@ From Undecidability.TM Require Import Single.StepTM Code.CodeTM TM mTM_to_TM Arb
 From Undecidability.StackMachines Require Import HaltSBTM_to_HaltBSM.
 From Undecidability.Shared.Libs.DLW Require Import vec pos sss subcode.
 From Undecidability Require Import bsm_utils bsm_defs.
+From Undecidability Require Import BSM_computable_to_MM_computable.
 
 Notation "v @[ t ]" := (Vector.nth v t) (at level 50).
 
@@ -75,7 +76,7 @@ Proof.
     Unshelve. reflexivity.
 Qed.
 
-Definition strpush_common (Σ : finType) (s b : Σ) :=
+Definition strpush_common_short (Σ : finType) (s b : Σ) :=
 encode_sym
   (projT1
      (projT2
@@ -107,7 +108,10 @@ true
                           (FinTypeEquiv.finite_n
                              (finType_CS
                                 (boundary + sigList (EncodeTapes.sigTape Σ)))))
-                       (inr (sigList_X (EncodeTapes.MarkedSymbol b)))) ++
+                       (inr (sigList_X (EncodeTapes.MarkedSymbol b)))).
+
+Definition strpush_common (Σ : finType) (s b : Σ) :=
+strpush_common_short s b ++
                   true
                   :: false :: nil.
 
@@ -122,36 +126,43 @@ Definition strpush_zero (Σ : finType) (s b : Σ) :=
                                        sigList (EncodeTapes.sigTape Σ)))))
                              (inr (sigList_X (EncodeTapes.RightBlank false)))).
 
-Lemma encode_bsm_zero (Σ : finType) n  s b :
-  { '( str1, n') | str1 = nil /\ forall (t : Vector.t (tape Σ) n),
-      encode_bsm Σ (encNatTM s b 0 ::: t) = 
-     [| str1 ++ (encode_bsm Σ t)@[Fin0]; (encode_bsm Σ t)@[Fin1]; strpush_zero s b ++ (skipn n' ((encode_bsm Σ t)@[Fin2])); (encode_bsm Σ t)@[Fin3] |]}.
+Lemma encode_bsm_at0 (Σ : finType) n (t : Vector.t (tape Σ) n) :
+   (encode_bsm Σ t) @[Fin0] = [].
 Proof.
-  eexists (_, _). split. shelve. cbn. intros t.
+  unfold encode_bsm, enc_tape, complete_encode, conv_tape.
+  destruct destruct_vector_cons as (? & ? & E). inv E. reflexivity.
+Qed.
+
+Lemma encode_bsm_at1 (Σ : finType) n :
+   forall (t : Vector.t (tape Σ) n), (encode_bsm Σ t) @[Fin1] = [false].
+Proof.
+  intros t.
+  unfold encode_bsm, enc_tape, complete_encode, conv_tape.
+  destruct destruct_vector_cons as (? & ? & E). inv E. reflexivity.
+Qed.
+
+Lemma encode_bsm_at3 (Σ : finType) n (t : Vector.t (tape Σ) n) :
+   (encode_bsm Σ t) @[Fin3] = [].
+Proof.
+  unfold encode_bsm, enc_tape, complete_encode, conv_tape.
+  destruct destruct_vector_cons as (? & ? & E). inv E. reflexivity.
+Qed.
+
+Lemma encode_bsm_zero (Σ : finType) s b :
+  { n' | forall n(t : Vector.t (tape Σ) n), (encode_bsm Σ (encNatTM s b 0 ::: t)) @[Fin2] = strpush_zero s b ++ (skipn n' ((encode_bsm Σ t)@[Fin2]))}.
+Proof.
+  eexists _. intros t.
   unfold encode_bsm at 1.
-  unfold enc_tape at 1. repeat f_equal.
-  - unfold complete_encode. unfold conv_tape.
-    etransitivity.
-    destruct destruct_vector_cons as (? & ? & E). inv E. cbn.
-    destruct_tapes. cbn. reflexivity.
-    symmetry. etransitivity.
-    destruct destruct_vector_cons as (? & ? & E). inv E. cbn.
-    destruct_tapes. cbn. reflexivity. instantiate (1 := []). reflexivity.
-  - unfold complete_encode, conv_tape.
-    etransitivity.
-    destruct destruct_vector_cons as (? & ? & E). inv E. cbn.
-    destruct_tapes. cbn. reflexivity.
-    destruct destruct_vector_cons as (? & ? & E). inv E. cbn. reflexivity.
-  - unfold complete_encode, conv_tape.
-    etransitivity.
-    destruct destruct_vector_cons as (? & ? & E). inv E. cbn - [skipn].
-    destruct_tapes. cbn - [skipn]. reflexivity.
-    symmetry. etransitivity.
-    destruct destruct_vector_cons as (? & ? & E). inv E. cbn - [skipn].
-    destruct_tapes. cbn - [skipn]. reflexivity.
-    rewrite skipn_app. 2: now rewrite length_encode_sym. unfold strpush_zero, strpush_common.
-    rewrite <- app_assoc. cbn. rewrite <- app_assoc. cbn. rewrite <- app_assoc. cbn. rewrite <- app_assoc. cbn. rewrite <- app_assoc. reflexivity.
-    Unshelve. reflexivity.
+  unfold enc_tape at 1. cbn.
+  unfold complete_encode, conv_tape.
+  etransitivity.
+  destruct destruct_vector_cons as (? & ? & E). inv E. cbn - [skipn].
+  destruct_tapes. cbn - [skipn]. reflexivity.
+  symmetry. etransitivity.
+  destruct destruct_vector_cons as (? & ? & E). inv E. cbn - [skipn].
+  destruct_tapes. cbn - [skipn]. reflexivity.
+  rewrite skipn_app. 2: now rewrite length_encode_sym. unfold strpush_zero, strpush_common, strpush_common_short.
+  rewrite <- app_assoc. cbn. rewrite <- app_assoc. cbn. rewrite <- app_assoc. cbn. rewrite <- app_assoc. cbn. rewrite <- app_assoc. reflexivity.
 Qed.
 
 Definition strpush_succ (Σ : finType) (s b : Σ) :=
@@ -165,43 +176,29 @@ strpush_common s b ++
                                        sigList (EncodeTapes.sigTape Σ)))))
                              (inr (sigList_X (EncodeTapes.UnmarkedSymbol s)))).
 
-Lemma encode_bsm_succ (Σ : finType) n m s b :
-  { '( str1, n') | str1 = nil /\ forall (t : Vector.t (tape Σ) n),
-      encode_bsm Σ (encNatTM s b (S m) ::: t) = 
-     [| str1 ++ (encode_bsm Σ (encNatTM s b m ::: t))@[Fin0]; (encode_bsm Σ (encNatTM s b m ::: t))@[Fin1]; strpush_succ s b ++ (skipn n' ((encode_bsm Σ (encNatTM s b m ::: t))@[Fin2])); (encode_bsm Σ (encNatTM s b m ::: t))@[Fin3] |]}.
+Lemma encode_bsm_succ (Σ : finType) n m s b (t : Vector.t (tape Σ) n) :
+      (encode_bsm Σ (encNatTM s b (S m) ::: t)) @[Fin2] = strpush_succ s b ++ (skipn (length (strpush_common_short s b)) ((encode_bsm Σ (encNatTM s b m ::: t))@[Fin2])).
 Proof.
-  eexists (_, _). split. shelve. cbn. intros t.
-  unfold encode_bsm at 1.
-  unfold enc_tape at 1. repeat f_equal.
-  - unfold complete_encode. unfold conv_tape.
-    etransitivity.
-    destruct destruct_vector_cons as (? & ? & E). inv E. cbn.
-    destruct_tapes. cbn. reflexivity.
-    symmetry. etransitivity.
-    destruct destruct_vector_cons as (? & ? & E). inv E. cbn.
-    destruct_tapes. cbn. reflexivity. instantiate (1 := []). reflexivity.
-  - unfold complete_encode, conv_tape.
-    etransitivity.
-    destruct destruct_vector_cons as (? & ? & E). inv E. cbn.
-    destruct_tapes. cbn. reflexivity.
-    destruct destruct_vector_cons as (? & ? & E). inv E. cbn. reflexivity.
-  - unfold complete_encode, conv_tape.
-    etransitivity.
-    destruct destruct_vector_cons as (? & ? & E). inv E. cbn - [skipn].
-    destruct_tapes. cbn - [skipn]. reflexivity.
-    symmetry. etransitivity.
-    destruct destruct_vector_cons as (? & ? & E). inv E. cbn - [skipn].
-    destruct_tapes. cbn - [skipn]. reflexivity.
-    match goal with [|- context [ skipn _ (?x1 ++ true :: false :: ?x2 ++ true :: false :: ?x3 ++ true :: false :: ?x4 ++ ?x5) ]] =>
-      replace (x1 ++ true :: false :: x2 ++ true :: false :: x3 ++ true :: false :: x4 ++ x5) with
-              ((x1 ++ true :: false :: x2 ++ true :: false :: x3 ++ true :: false :: x4) ++ x5)
-    end.    
-    rewrite skipn_app. 2: reflexivity.
-    2:{ rewrite <- app_assoc. cbn. rewrite <- app_assoc. cbn. rewrite <- app_assoc. cbn. reflexivity. }
-
-    unfold strpush_succ, strpush_common.
-    rewrite <- app_assoc. cbn. rewrite <- app_assoc. cbn. rewrite <- app_assoc. cbn. rewrite <- app_assoc. cbn. rewrite <- app_assoc. cbn. reflexivity.
-    Unshelve. reflexivity.
+  unfold encode_bsm.
+  unfold enc_tape. repeat f_equal.
+  unfold complete_encode, conv_tape.
+  etransitivity.
+  destruct destruct_vector_cons as (? & ? & E). cbn - [skipn]. inv E. cbn - [skipn].
+  unfold strpush_common, strpush_common_short.
+  destruct_tapes. cbn - [skipn]. reflexivity. 
+  unfold strpush_common, strpush_common_short. cbn - [skipn].
+  
+  symmetry. etransitivity. cbn - [skipn].
+  destruct destruct_vector_cons as (? & ? & E). inv E. cbn - [skipn].
+  destruct_tapes. cbn - [skipn]. reflexivity. 
+  match goal with [|- context [ skipn _ (?x1 ++ true :: false :: ?x2 ++ true :: false :: ?x3 ++ true :: false :: ?x4 ++ ?x5) ]] =>
+    replace (x1 ++ true :: false :: x2 ++ true :: false :: x3 ++ true :: false :: x4 ++ x5) with
+            ((x1 ++ true :: false :: x2 ++ true :: false :: x3 ++ true :: false :: x4) ++ x5)
+  end.    
+  rewrite skipn_app. 2:{ reflexivity. }
+  2:{ rewrite <- app_assoc. cbn. rewrite <- app_assoc. cbn. rewrite <- app_assoc. cbn. reflexivity. }
+  unfold strpush_succ, strpush_common, strpush_common_short.
+  rewrite <- app_assoc. cbn. rewrite <- app_assoc. cbn. rewrite <- app_assoc. cbn. rewrite <- app_assoc. cbn. rewrite <- app_assoc. cbn. reflexivity.
 Qed.
 
 Lemma BSM_complete_simulation' n Σ (M : TM Σ n) m m' i :
@@ -234,6 +231,289 @@ Proof.
   exists P. split. exact H1.
   intros t v'' v''' ([out1 out2] & H % BSM_sss.eval_iff). eapply H2. eauto.
 Qed. 
+
+Local Notation "P // s ->> t" := (sss_compute (@bsm_sss _) P s t).
+
+Lemma vec_app_spec {X n m} (v : Vector.t X n) (w : Vector.t X m) :
+  vec_app v w = Vector.append v w.
+Proof.
+  induction v.
+  - cbn. eapply vec_pos_ext. intros. now rewrite vec_pos_set.
+  - rewrite vec_app_cons. cbn. congruence.
+Qed.
+
+Lemma pos_right_left {n m} p q :
+@pos_left n m p <> @pos_right n m q.
+Proof.
+induction n; cbn.
+- inversion p.
+- eapply (Fin.caseS' p).
+  + cbn. congruence.
+  + cbn. intros ? ? % pos_nxt_inj. firstorder.
+Qed.
+
+Lemma pos_left_right {n m} p q :
+@pos_right n m q <> @pos_left n m p.
+Proof.
+induction n; cbn.
+- inversion p.
+- eapply (Fin.caseS' p).
+  + cbn. congruence.
+  + cbn. intros ? ? % pos_nxt_inj. firstorder.
+Qed.
+Hint Immediate pos_left_right pos_right_left : core.
+
+Lemma pos_right_inj {n m} p q :
+  @pos_right n m p = @pos_right n m q -> p = q.
+Proof.
+  induction n in p, q |- *; cbn in *. 
+  - eauto.
+  - intros. eapply IHn, pos_nxt_inj, H.
+Qed.
+
+Lemma vec_pos_const {k} {X x} (p : pos k) : vec_pos (@Vector.const X x k) p = x.
+Proof.
+  induction p; cbn; eauto.
+Qed.
+
+Lemma vec_pos_spec {k} {X} (p : pos k) (v : Vector.t X k) : vec_pos v p = Vector.nth v p.
+Proof.
+  induction v in p |- *.
+  - inversion p.
+  - eapply (Fin.caseS' p).
+    + reflexivity.
+    + intros. cbn. eauto.
+Qed.
+
+Lemma Fin4_cases (P : pos 4 -> Prop) :
+   P Fin0 -> P Fin1 -> P Fin2 -> P Fin3 -> forall p, P p.
+Proof.
+  intros H0 H1 H2 H3. 
+  repeat (intros p; eapply (Fin.caseS' p); clear p; [ eauto | ]).
+  intros p. inversion p.
+Qed.
+
+Lemma PREP1_spec k Σ  : 
+{ PREP1 : list (bsm_instr ((1 + k) + 4)) | forall v : Vector.t nat k, 
+    (0, PREP1) // (0, Vector.append ([] ::: Vector.map (fun n0 : nat => repeat true n0) v) (Vector.const [] 4)) ->>
+                  (length PREP1, Vector.append ([] ::: Vector.map (fun n0 : nat => repeat true n0) v) ((@encode_bsm Σ _ (Vector.const niltape 4)))) }.
+Proof.
+  exists (push_exactly (pos_right (1 + k) Fin0) ((@encode_bsm Σ _ (Vector.const niltape 4))@[Fin0])
+       ++ push_exactly (pos_right (1 + k) Fin1) ((@encode_bsm Σ _ (Vector.const niltape 4))@[Fin1])
+       ++ push_exactly (pos_right (1 + k) Fin2) ((@encode_bsm Σ _ (Vector.const niltape 4))@[Fin2])
+       ++ push_exactly (pos_right (1 + k) Fin3) ((@encode_bsm Σ _ (Vector.const niltape 4))@[Fin3])).
+  intros v.
+  eapply subcode_sss_compute_trans. 2: eapply (push_exactly_spec (pos_right (1 + k) Fin0) 0 ((@encode_bsm Σ _ (Vector.const niltape 4))@[Fin0])). 1:auto.
+  eapply subcode_sss_compute_trans. 2: eapply (push_exactly_spec (pos_right (1 + k) Fin1) _ ((@encode_bsm Σ _ (Vector.const niltape 4))@[Fin1])). 1:auto.
+  eapply subcode_sss_compute_trans. 2: eapply (push_exactly_spec (pos_right (1 + k) Fin2) _ ((@encode_bsm Σ _ (Vector.const niltape 4))@[Fin2])). 1:auto.
+  eapply subcode_sss_compute_trans. 2: eapply (push_exactly_spec (pos_right (1 + k) Fin3) _ ((@encode_bsm Σ _ (Vector.const niltape 4))@[Fin3])). 1:auto.
+  bsm sss stop. f_equal.
+  1:rewrite !app_length; lia.
+  eapply vec_pos_ext. eapply pos_left_right_rect. 
+  - rewrite <- !vec_app_spec. symmetry. rewrite vec_pos_app_left.
+    rewrite !vec_change_neq; auto.
+    now rewrite vec_pos_app_left.
+  - rewrite <- !vec_app_spec. rewrite !vec_pos_app_right. 
+    intros p; eapply (Fin.caseS' p); clear p.
+    1:{ repeat (rewrite vec_change_neq; [ | intros ? % pos_right_inj; congruence]).
+        rewrite vec_change_eq; [ | auto]. rewrite vec_pos_app_right.
+        now rewrite vec_pos_const, app_nil_r, vec_pos_spec. }
+    intros p; eapply (Fin.caseS' p); clear p.
+    1:{ rewrite vec_change_neq; [ | intros ? % pos_right_inj % pos_nxt_inj; congruence].
+        rewrite vec_change_neq; [ | intros ? % pos_right_inj % pos_nxt_inj; congruence].
+        rewrite vec_change_eq; [ | auto]. rewrite vec_pos_app_right.
+        rewrite vec_pos_const. rewrite vec_change_neq; [ | intros ? % pos_right_inj; congruence].
+        rewrite vec_pos_app_right. now rewrite vec_pos_const, app_nil_r, vec_pos_spec. }
+    intros p; eapply (Fin.caseS' p); clear p.
+    1:{ rewrite vec_change_neq; [ | intros ? % pos_right_inj % pos_nxt_inj % pos_nxt_inj; congruence].
+        rewrite vec_change_eq; [ | auto]. rewrite vec_pos_app_right.
+        rewrite vec_pos_const. rewrite vec_change_neq; [ | intros ? % pos_right_inj % pos_nxt_inj; congruence].
+        rewrite vec_change_neq; [ | intros ? % pos_right_inj; congruence].
+        rewrite vec_pos_app_right. now rewrite vec_pos_const, app_nil_r, vec_pos_spec. }
+    intros p; eapply (Fin.caseS' p); clear p.
+    1:{ rewrite vec_change_eq; [ | auto]. rewrite vec_pos_app_right.
+        rewrite vec_pos_const. rewrite vec_change_neq; [ | intros ? % pos_right_inj % pos_nxt_inj % pos_nxt_inj; congruence].
+        rewrite vec_change_neq; [ | intros ? % pos_right_inj % pos_nxt_inj; congruence].
+        rewrite vec_change_neq; [ | intros ? % pos_right_inj; congruence].
+        rewrite vec_pos_app_right. now rewrite vec_pos_const, app_nil_r, vec_pos_spec. }
+    intros p. inversion p.
+Qed.
+
+Lemma vec_map_spec {X Y n} (v : Vector.t X n) (f : X -> Y) :
+  vec_map f v = Vector.map f v.
+Proof.
+  induction v; cbn; congruence.
+Qed.
+
+Lemma pos_left_inj {n m} p q :
+  @pos_left n m p = @pos_left n m q -> p = q.
+Proof.
+  induction p in q |- *; cbn in *. 
+  - eapply (Fin.caseS' q).
+    + reflexivity.
+    + clear q. cbn. congruence.
+  - eapply (Fin.caseS' q).
+    + cbn. congruence.
+    + clear q. cbn. intros. f_equal. eapply IHp.
+      now eapply pos_nxt_inj.
+Qed.
+
+Lemma PREP2_spec'' k (Σ : finType) (x : pos k) i s b : 
+{ PREP2 : list (bsm_instr ((1 + k) + 4)) | length PREP2 = 2 + (length (strpush_common_short s b)) + length ((strpush_succ s b)) /\
+forall v : Vector.t (list bool) k,  forall n, forall t : Vector.t (tape Σ) n, forall m m',
+   v @[x] = repeat true m ->
+    (i, PREP2) // (i,                Vector.append ([] ::: v) ((@encode_bsm Σ _ (encNatTM s b m' ::: t)))) ->>
+                  (i + length PREP2, Vector.append ([] ::: vec_change v x nil) ((@encode_bsm Σ _ (encNatTM s b (m + m') ::: t)))) }.
+Proof.
+  exists (POP (pos_left 4 (pos_right 1 x)) 0 (i + 2 + (length (strpush_common_short s b)) + length ((strpush_succ s b)))
+       :: pop_many (pos_right (1 + k) Fin2) (length (strpush_common_short s b)) (1 + i)
+       ++ push_exactly (pos_right (1 + k) Fin2) (strpush_succ s b)
+       ++ POP (pos_left 4 Fin0) 0 i :: nil). split.
+  { cbn. rewrite !app_length. cbn. rewrite pop_many_length, push_exactly_length. lia. }
+  intros v n t m m' Hx.
+  induction m in v, m', Hx |- *.
+  - bsm sss POP empty with (pos_left 4 (pos_right 1 x)) 0 (i + 2 + (length (strpush_common_short s b)) + length ((strpush_succ s b))).
+    rewrite <- !vec_app_spec, vec_pos_app_left. cbn in *. 
+    rewrite vec_pos_spec, Hx. reflexivity.
+    bsm sss stop. f_equal. cbn. rewrite !app_length. cbn. rewrite pop_many_length, push_exactly_length. lia. cbn in Hx.
+    rewrite <- Hx. now rewrite <- vec_pos_spec, vec_change_same.
+  - bsm sss POP 1 with (pos_left 4 (pos_right 1 x)) 0 (i + 2 + (length (strpush_common_short s b)) + length ((strpush_succ s b))) (repeat true m).
+    1:{ rewrite <- !vec_app_spec, vec_pos_app_left. cbn.
+        rewrite vec_pos_spec, Hx. reflexivity. }
+    eapply subcode_sss_compute_trans. 2: eapply (pop_many_spec (pos_right (1 + k) Fin2) (length (strpush_common_short s b)) (1 + i)). 1:auto.
+    eapply subcode_sss_compute_trans. 2: eapply (push_exactly_spec (pos_right (1 + k) Fin2) _ (strpush_succ s b)).
+    { eexists (POP _ _ _ :: pop_many _ _ _), ([POP _ _ _]). split. 
+      simpl_list. cbn. simpl_list. reflexivity.
+      cbn; rewrite pop_many_length. lia.
+    }
+    bsm sss POP empty with (pos_left 4 Fin0) 0 i. {
+      eexists (POP _ _ _ :: pop_many _ _ _ ++ push_exactly _ _), []. simpl_list. cbn. simpl_list. cbn. split. reflexivity.
+      rewrite pop_many_length, push_exactly_length. lia. }
+    specialize IHm with (m' := (S m')). replace (S m + m') with (m + S m') by lia.
+    match goal with [ |- sss_compute _ _ (_, ?st) _ ] => evar (ev : Vector.t (list bool) ((1 + k) + 4)); enough (st = ev) as ->; subst ev end.
+    match goal with [ |- sss_compute _ _ _ (_, ?st) ] => evar (ev : Vector.t (list bool) ((1 + k) + 4)); enough (st = ev) as ->; subst ev end.
+    eapply IHm with (v := vec_change v x (repeat true m)). now rewrite <- vec_pos_spec, vec_change_eq. now rewrite vec_change_idem.
+    rewrite <- !vec_app_spec.
+    eapply vec_pos_ext. eapply pos_left_right_rect. 
+    + symmetry. rewrite vec_pos_app_left.
+      rewrite vec_change_neq; auto.
+      rewrite vec_change_neq; auto. cbn in p.
+      eapply (Fin.caseS' p); clear p. cbn. reflexivity.
+      intros p. 
+      destruct (pos_eq_dec p x).
+      * rewrite vec_change_eq. 2: now subst. cbn. subst. now rewrite vec_change_eq.
+      * rewrite vec_change_neq. 2: intros ? % pos_left_inj % pos_nxt_inj; eauto.
+        rewrite vec_pos_app_left.  cbn. rewrite vec_change_neq; eauto.
+    + intros p. symmetry. rewrite !vec_pos_app_right. symmetry.
+      rewrite !vec_change_idem.
+      revert p. 
+      apply Fin4_cases.
+      * repeat (rewrite vec_change_neq; [ | intros ? % pos_right_inj; congruence]).
+          rewrite vec_change_neq; [ | eapply pos_right_left]. rewrite vec_pos_app_right.
+          now rewrite !vec_pos_spec, !encode_bsm_at0.
+      * rewrite vec_change_neq; [ | intros ? % pos_right_inj % pos_nxt_inj; congruence].
+        rewrite vec_change_neq; [ | auto].
+        now rewrite vec_pos_app_right, !vec_pos_spec, !encode_bsm_at1.
+      * rewrite vec_change_eq; auto.
+        rewrite vec_change_eq; eauto.
+        rewrite vec_change_neq; eauto.
+        rewrite vec_pos_app_right.
+        now rewrite !vec_pos_spec, encode_bsm_succ.
+      * rewrite vec_change_neq; [ | intros ? % pos_right_inj % pos_nxt_inj % pos_nxt_inj; congruence].
+        rewrite vec_change_neq; [ | auto]. 
+        now rewrite vec_pos_app_right, !vec_pos_spec, !encode_bsm_at3.
+Qed.
+
+Definition PREP2''_length (Σ : finType) (s b : Σ) := proj1_sig (encode_bsm_zero s b) + length (strpush_zero s b) + 2 + (length (strpush_common_short s b)) + length ((strpush_succ s b)).
+
+Lemma PREP2_spec' k (Σ : finType) (x : pos k) i s b n : 
+{ PREP2 : list (bsm_instr ((1 + k) + 4)) | length PREP2 = PREP2''_length s b  /\
+forall v : Vector.t (list bool) k, forall t : Vector.t (tape Σ) n, forall m,
+   v @[x] = repeat true m ->
+    (i, PREP2) // (i,                Vector.append ([] ::: v) ((@encode_bsm Σ _ t))) ->>
+                  (i + length PREP2, Vector.append ([] ::: vec_change v x nil) ((@encode_bsm Σ _ (encNatTM s b m ::: t)))) }.
+Proof.
+  unfold PREP2''_length. 
+  destruct (encode_bsm_zero s b) as [n' Hn'].
+  destruct (PREP2_spec'' x (i + n' + length (strpush_zero s b)) s b) as [PREP2 [Hl2 H]].
+  exists (pop_many (pos_right (1 + k) Fin2) n' i 
+       ++ push_exactly (pos_right (1 + k) Fin2) (strpush_zero s b)
+       ++ PREP2). split.
+  {  cbn. rewrite !app_length. cbn. rewrite pop_many_length, push_exactly_length. cbn in Hl2. rewrite Hl2. lia. }
+  intros v t m Hm.
+  eapply subcode_sss_compute_trans. 2: eapply (pop_many_spec (pos_right (1 + k) Fin2) n' i). 1:auto.
+  eapply subcode_sss_compute_trans. 2: eapply (push_exactly_spec (pos_right (1 + k) Fin2) _ (strpush_zero s b)). 
+  { eexists (pop_many _ _ _), PREP2. split. reflexivity. rewrite pop_many_length. lia. }
+  specialize H with (m' := 0) (v := v) (1 := Hm). replace (m + 0) with m in H by lia.
+  eapply subcode_sss_compute_trans. 2:{
+  match goal with [ |- sss_compute _ _ (_, ?st) _ ] => evar (ev : Vector.t (list bool) ((1 + k) + 4)); enough (st = ev) as ->; subst ev end.
+  match goal with [ |- sss_compute _ _ (?st, _) _ ] => evar (ev : nat); enough (st = ev) as ->; subst ev end.
+  - eapply H. 
+  - rewrite push_exactly_length. lia.
+  - eapply vec_pos_ext. eapply pos_left_right_rect.
+    + intros p. rewrite <- !vec_app_spec, !vec_pos_app_left.
+      rewrite vec_change_neq; auto.
+      rewrite vec_change_neq; auto. now rewrite vec_pos_app_left.
+    + rewrite <- !vec_app_spec. eapply Fin4_cases.
+      * rewrite vec_change_neq; [ | intros ? % pos_right_inj; congruence].
+        rewrite vec_change_neq; [ | intros ? % pos_right_inj; congruence].
+        rewrite !vec_pos_app_right.
+        rewrite !vec_pos_spec. now rewrite !encode_bsm_at0.
+      * rewrite vec_change_neq; [ | intros ? % pos_right_inj % pos_nxt_inj; congruence].
+        rewrite vec_change_neq; [ | intros ? % pos_right_inj % pos_nxt_inj; congruence].
+        now rewrite !vec_pos_app_right, !vec_pos_spec, !encode_bsm_at1.
+      * rewrite vec_change_eq; auto.
+        rewrite vec_change_eq; eauto.
+        rewrite !vec_pos_app_right.
+        now rewrite !vec_pos_spec, Hn'.
+      * rewrite vec_change_neq; [ | intros ? % pos_right_inj % pos_nxt_inj % pos_nxt_inj; congruence].
+        rewrite vec_change_neq; [ | intros ? % pos_right_inj % pos_nxt_inj % pos_nxt_inj; congruence].
+        now rewrite !vec_pos_app_right, !vec_pos_spec, !encode_bsm_at3.
+  }
+  { eexists (pop_many _ _ _ ++ push_exactly _ _), []. rewrite app_nil_r. split. now simpl_list. rewrite app_length, pop_many_length, push_exactly_length. lia. }
+  bsm sss stop. f_equal.
+  rewrite !app_length, pop_many_length, push_exactly_length. lia.
+Qed.
+
+Fixpoint PREP2' (Σ : finType) (s b : Σ) k (k' : nat) (H : k' <= k) (i : nat) : list (bsm_instr ((1 + k) + 4)).
+Proof.
+  destruct k'.
+  - exact List.nil.
+  - refine (List.app (PREP2' Σ s b k k' _ i) _). abstract lia.
+    assert (Hn : k' < k) by abstract lia.
+    refine (proj1_sig (@PREP2_spec' k Σ (Fin.of_nat_lt Hn) (14 * k' + i) s b (k' + 4))).
+Defined.
+
+Lemma PREP2'_length (Σ : finType) (s b : Σ) k (k' : nat) (H : k' <= k) (i : nat) :
+  | @PREP2' Σ s b k k' H i | = k' * PREP2''_length s b.
+Proof.
+  induction k' in k, H, i |- *.
+  - cbn. reflexivity.
+  - cbn - [mult]. destruct PREP2_spec' as (? & ? & ?). cbn. rewrite app_length. cbn in e. rewrite e. cbn in IHk'. rewrite IHk'. lia.
+Qed.
+
+Notation "v1 +++ v2" := (Vector.append v1 v2) (at level 60).
+
+Lemma PREP2_spec_strong k (Σ : finType) (x : pos k) i s b k' k'' v (v' : Vector.t nat k') (t : Vector.t (tape Σ) 4) : 
+  forall H,
+    (i, @PREP2' Σ s b (k'' + k') k'' H  i) //
+        (i,                                   ([] ::: Vector.map (fun n => repeat true n) v +++ Vector.const [] k') +++  (@encode_bsm Σ _ (Vector.map (encNatTM s b) v' +++ t))) ->>
+        (i + length(@PREP2' Σ s b (k'' + k') k'' H  i), ([] ::: Vector.const [] (k'' + k')                                    +++  (@encode_bsm Σ _ (Vector.map (encNatTM s b) (v +++ v') +++ t)))).
+Proof.
+  intros H. induction k'' in k', H, v, v', i |- *.
+  - cbn. bsm sss stop. f_equal. lia. f_equal. revert v. eapply (Vector.case0). cbn. reflexivity.
+  - cbn - [mult]. 
+    edestruct (vector_inv_back v) as [(y, vl) Hv]. cbn - [mult].
+    eapply subcode_sss_compute_trans with (P := (i, _)). { eexists [], _. cbn - [mult]. split. reflexivity. cbn; now rewrite NPeano.Nat.add_0_r. } 
+    { cbn - [mult] in IHk''. specialize (IHk'' i (S k') vl (y ::: v')).
+      generalize (@PREP2'_subproof (S (k'' + k')) k'' H).
+      replace (S (k'' + k')) with (k'' + S k').
+      unshelve epose proof (IHk'' _). astract lia.
+      
+      match goal with [ |- sss_compute _ _ (_, ?st) _ ] => evar (ev : vec (list bool) (S (S (k'' + k' + 4)))); enough (st = ev) as ->; subst ev end. eapply IHk''.
+      
+    specialize IHk'' with (v := vl) (v' := y ::: v').
+  
 
 Lemma PREP_spec m k n Σ s b :
   { PREP | forall v : Vector.t nat k,
